Semantics/Stlc/Rewrite.lean
@@ -2,37 +2,37 @@ import Semantics.Stlc.Lang
 import Mathlib.Logic.Relation
 
 def value: Term → Bool
-  | Term.abs _ _ _ | Term.tt | Term.ff => true
+  | Λ _:_↦_ | ⊤ | ⊥ => true
   | _ => false
 
 def subst (x: String) (s: Term) (t: Term): Term :=
   match t with
   | Term.var y => bif x = y then s else t
-  | Term.abs y T t₁ => bif x = y then t else Term.abs y T (subst x s t₁)
-  | Term.app t₁ t₂ => Term.app (subst x s t₁) (subst x s t₂)
-  | Term.cond t₁ t₂ t₃ => Term.cond (subst x s t₁) (subst x s t₂) (subst x s t₃)
+  | Λ y:T↦t₁ => bif x = y then t else Λ y:T↦(subst x s t₁)
+  | t₁..t₂ => (subst x s t₁)..(subst x s t₂)
+  | t₁ ? t₂ | t₃ => (subst x s t₁) ? subst x s t₂ | subst x s t₃
   | otherwise => otherwise
 
 notation "[" x "≔" s "]" t => subst x s t
 
 inductive step: Term → Term → Prop where
   | appabs (h: value v):
-    step (Term.app (Term.abs x _ t) v) ([x ≔ v]t)
+    step ((Λ x:_ ↦ t)..v) ([x ≔ v]t)
 
   | app₁ (h₁: step t t'):
-    step (Term.app t u) (Term.app t' u)
+    step (t..u) (t'..u)
 
   | app₂ (h₁: value v) (h₂: step u u'):
-    step (Term.app v u) (Term.app v u')
+    step (v..u) (v..u')
 
   | cond₁:
-    step (Term.cond tt t _) t
+    step (⊤ ? t | _) t
 
   | cond₂:
-    step (Term.cond ff _ u) u
+    step (⊥ ? _ | u) u
 
   | cond₃ (h: step b b'):
-    step (Term.cond b t u) (Term.cond b' t u)
+    step (b ? t | u) (b' ? t | u)
 
 infix:100 " ⇒ " => step
 
