Semantics/Stlc/Typing.lean
@@ -4,37 +4,37 @@ import Mathlib.Logic.Function.Basic
 def Context := String → Option Ty
 def empty_ctx: Context := λ _ ↦ none
 
-inductive HasTy: Context → Term → Ty → Prop where
+inductive has_type: Context → Term → Ty → Prop where
   | var (h: Γ x = some T):
-    HasTy Γ (Term.var x) T
-  | abs (h: HasTy (Function.update Γ x (some T₂)) t T₁):
-    HasTy Γ (Term.abs x T₂ t) (Ty.Arrow T₂ T₁)
-  | app (h₁: HasTy Γ t₁ (Ty.Arrow T₂ T₁)) (h₂: HasTy Γ t₂ T₂):
-    HasTy Γ (Term.app t₁ t₂) T₁
-  | true:
-    HasTy Γ Term.tt Ty.Bool
-  | false:
-    HasTy Γ Term.ff Ty.Bool
-  | cond (h₁: HasTy Γ b Ty.Bool) (h₂: HasTy Γ t₁ T₁) (h₃: HasTy Γ t₂ T₁):
-    HasTy Γ (Term.cond b t₁ t₂) T₁
+    has_type Γ (Term.var x) T
+  | abs (h: has_type (Function.update Γ x (some T₂)) t T₁):
+    has_type Γ (Λ x:T₂ ↦ t) (T₂ → T₁)
+  | app (h₁: has_type Γ t₁ (T₂ → T₁)) (h₂: has_type Γ t₂ T₂):
+    has_type Γ (t₁..t₂) T₁
+  | tt:
+    has_type Γ ⊤ 𝔹
+  | ff:
+    has_type Γ ⊥ 𝔹
+  | cond (h₁: has_type Γ b 𝔹) (h₂: has_type Γ t₁ T₁) (h₃: has_type Γ t₂ T₁):
+    has_type Γ (b ? t₁ | t₂) T₁
 
-notation Γ " ⊢ " t " : " T => HasTy Γ t T
+notation Γ " ⊢ " t " : " T => has_type Γ t T
 
 theorem typing_example_1:
-  empty_ctx ⊢ ⦃λx:Bool↦x⦄ : ⦃Bool → Bool⦄ := HasTy.abs (HasTy.var rfl)
+  empty_ctx ⊢ ⦃Λ x:𝔹 ↦ x⦄ : ⦃𝔹 → 𝔹⦄ := has_type.abs (has_type.var rfl)
 
 /-
 ## Canonical forms
 -/
 
 theorem canonical_form_bool
-  (h₁: empty_ctx ⊢ t : Ty.Bool) (h₂: value t):
-  (t = Term.tt) ∨ (t = Term.ff) :=
+  (h₁: empty_ctx ⊢ t : 𝔹) (h₂: value t):
+  (t = ⊤) ∨ (t = ⊥) :=
   by cases h₁ <;> cases h₂ <;> simp
 
 theorem canonical_form_fun
-  (h₁: empty_ctx ⊢ t : (Ty.Arrow T₁ T₂)) (h₂: value t):
-  ∃x u, t = (Term.abs x T₁ u) :=
+  (h₁: empty_ctx ⊢ t : (T₁ → T₂)) (h₂: value t):
+  ∃x u, t = Λ x : T₁ ↦ u :=
   by cases h₁ <;> cases h₂; simp
 
 /-
@@ -49,7 +49,7 @@ theorem progress (h: empty_ctx ⊢ t : T):
     . rename_i h; cases h
     . exact Or.inl rfl
     . simp at *
-      rename_i t₁ _ _ t₂ h₁ h₂ ih₁ ih₂
+      rename_i t₁ _ _ t₂ h₁ _ ih₁ ih₂
       apply Or.inr
       cases ih₁ with
       | inl h =>
@@ -63,13 +63,31 @@ theorem progress (h: empty_ctx ⊢ t : T):
               rw [hc]
               exists [x≔t₂]w
               exact step.appabs hh
-        | inr h => {
-          sorry
-        }
+        | inr hh =>
+          cases hh with
+          | intro w hh =>
+            exists t₁..w
+            exact step.app₂ h hh
       | inr h =>
         cases h with
         | intro w h =>
           exists (Term.app w t₂)
           apply step.app₁ h
-
+    . exact Or.inl rfl
+    . exact Or.inl rfl
+    . simp at *
+      rename_i t₁ _ t₂ h₁ _ _ ih₁ _ _
+      cases ih₁ with
+      | inl hh =>
+        apply Or.inr
+        have hc := canonical_form_bool h₁ hh
+        cases hc with
+        | inl hc => exists t₁; rw [hc]; exact step.cond₁
+        | inr hc => exists t₂; rw [hc]; exact step.cond₂
+      | inr hh =>
+        apply Or.inr
+        cases hh with
+        | intro w hh =>
+          exists w ? t₁ | t₂
+          exact step.cond₃ hh
   }
