Semantics/Stlc/Lang.lean
@@ -10,34 +10,48 @@ inductive Term where
   | ff
   | cond: Term → Term → Term → Term
 
+
+
 -- Syntax of the language
 declare_syntax_cat stlc
 
 syntax "(" stlc ")" : stlc
 syntax ident: stlc
 -- stmt
-syntax "λ" ident ":" stlc "↦" stlc : stlc
-syntax "if " stlc " then " stlc " else " stlc : stlc
+syntax "Λ" ident ":" stlc "↦" stlc : stlc
+syntax stlc "?" stlc "|" stlc : stlc
 syntax stlc " → " stlc : stlc
-syntax stlc stlc : stlc
+syntax stlc ".." stlc : stlc
+syntax "⊤": stlc
+syntax "⊥": stlc
+syntax "𝔹": stlc
+
 -- meta
 syntax "⦃" stlc "⦄" : term
 
 macro_rules
   -- keywords
-  | `(⦃true⦄)   => `(Term.tt)
-  | `(⦃false⦄)  => `(Term.ff)
-  | `(⦃Bool⦄)   => `(Ty.Bool)
+  | `(⦃⊤⦄)   => `(Term.tt)
+  | `(⦃⊥⦄)  => `(Term.ff)
+  | `(⦃𝔹⦄)   => `(Ty.Bool)
   | `(⦃$x → $y⦄) => `(Ty.Arrow ⦃$x⦄ ⦃$y⦄)
   -- general
   | `(⦃($x)⦄) => `(⦃$x⦄)
   | `(⦃$x:ident⦄) => `(Term.var $(Lean.quote (toString x.getId)))
   -- stlc
-  | `(⦃λ $x : $t ↦ $e⦄) => `(Term.abs $(Lean.quote (toString x.getId)) ⦃$t⦄ ⦃$e⦄)
-  | `(⦃$x $y⦄) => `(Term.app ⦃$x⦄ ⦃$y⦄)
-  | `(⦃if $b then $x else $y⦄) => `(Term.cond ⦃$b⦄ ⦃$x⦄ ⦃$y⦄)
+  | `(⦃Λ $x : $t ↦ $e⦄) => `(Term.abs $(Lean.quote (toString x.getId)) ⦃$t⦄ ⦃$e⦄)
+  | `(⦃$x..$y⦄) => `(Term.app ⦃$x⦄ ⦃$y⦄)
+  | `(⦃$b ? $x | $y⦄) => `(Term.cond ⦃$b⦄ ⦃$x⦄ ⦃$y⦄)
 
 
-#check ⦃(λx:Bool↦x) true⦄
-#check ⦃(λx:Bool↦if x then false else true) true⦄
-#check ⦃λf:Bool→Bool↦f (f true)⦄
+#check ⦃(Λ x: 𝔹 ↦x)..⊤⦄
+#check ⦃(Λ x: 𝔹 ↦ x ? ⊥ | ⊤)..⊤⦄
+#check ⦃Λ f: 𝔹 → 𝔹 ↦ f..(f..⊤)⦄
+
+notation "Λ " x ": " T " ↦ " t => Term.abs x T t
+infix:100 ".." => Term.app
+notation b " ? " a " | " c => Term.cond b a c
+notation "⊤" => Term.tt
+notation "⊥" => Term.ff
+infix:100 "→" => Ty.Arrow
+notation "𝔹" => Ty.Bool
